refactor for v4.27

ffi/basic.c
@@ -1,0 +1,167 @@
+#include "ffi.h"
+#include <string.h>
+#include <lean/lean.h>
+#include <sodium.h>
+
+LEAN_EXPORT lean_obj_res lean_sodium_init(lean_obj_arg world) {
+  if (sodium_init() < 0) {
+    return lean_io_result_mk_error(lean_mk_io_user_error(lean_mk_string("Failed to initialize LibSodium")));
+  }
+  return lean_io_result_mk_ok(lean_box(0));
+}
+
+LEAN_EXPORT lean_obj_res lean_sodium_malloc(b_lean_obj_arg tau, size_t size, lean_obj_arg world) {
+  void* ptr = sodium_malloc(size);
+  randombytes_buf(ptr, size);
+  sodium_mprotect_noaccess(ptr);
+  lean_object* ret = lean_alloc_ctor(0, 1, sizeof(size_t));
+  lean_ctor_set(ret, 0, secure_obj_to_lean(ptr));
+  lean_ctor_set_usize(ret, 1, size);
+  return lean_io_result_mk_ok(ret);
+}
+
+LEAN_EXPORT lean_obj_res lean_sodium_malloc_deterministic(b_lean_obj_arg tau, size_t size, b_lean_obj_arg seed, lean_obj_arg world) {
+  void* ptr = sodium_malloc(size);
+  randombytes_buf_deterministic(ptr, size, lean_sarray_cptr(seed));
+  sodium_mprotect_noaccess(ptr);
+  lean_object* ret = lean_alloc_ctor(0, 1, sizeof(size_t));
+  lean_ctor_set(ret, 0, secure_obj_to_lean(ptr));
+  lean_ctor_set_usize(ret, 1, size);
+  return lean_io_result_mk_ok(ret);
+}
+
+LEAN_EXPORT uint8_t lean_sodium_secure_obj_is_zero(b_lean_obj_arg tau, size_t size, b_lean_obj_arg obj) {
+  void* ptr = secure_obj_of_lean(lean_ctor_get(obj, 0));
+  sodium_mprotect_readonly(ptr);
+  int ret = sodium_is_zero(ptr, size);
+  sodium_mprotect_noaccess(ptr);
+  return ret == 1;
+}
+
+LEAN_EXPORT uint8_t lean_sodium_secure_obj_compare(b_lean_obj_arg tau, size_t size, b_lean_obj_arg obj1, b_lean_obj_arg obj2) {
+  void* ptr1 = secure_obj_of_lean(lean_ctor_get(obj1, 0));
+  void* ptr2 = secure_obj_of_lean(lean_ctor_get(obj2, 0));
+  sodium_mprotect_readonly(ptr1);
+  sodium_mprotect_readonly(ptr2);
+  int ret = sodium_compare(ptr1, ptr2, size);
+  sodium_mprotect_noaccess(ptr1);
+  sodium_mprotect_noaccess(ptr2);
+  return ret + 1;
+}
+
+LEAN_EXPORT lean_obj_res lean_sodium_randombytes_buf(b_lean_obj_arg tau, size_t size, lean_obj_arg world) {
+  void* ptr = sodium_malloc(size);
+  randombytes_buf(ptr, size);
+  sodium_mprotect_readonly(ptr);
+  lean_object* ret = lean_alloc_ctor(0, 1, 2 * sizeof(size_t));
+  lean_ctor_set(ret, 0, secure_obj_to_lean(ptr));
+  lean_ctor_set_usize(ret, 1, 0);
+  lean_ctor_set_usize(ret, 2, size);
+  return lean_io_result_mk_ok(ret);
+}
+
+LEAN_EXPORT lean_obj_res lean_sodium_randombytes_buf_deterministic(b_lean_obj_arg tau, size_t size, b_lean_obj_arg seed, lean_obj_arg world) {
+  void* ptr = sodium_malloc(size);
+  randombytes_buf_deterministic(ptr, size, lean_sarray_cptr(seed));
+  sodium_mprotect_readonly(ptr);
+  lean_object* ret = lean_alloc_ctor(0, 1, 2 * sizeof(size_t));
+  lean_ctor_set(ret, 0, secure_obj_to_lean(ptr));
+  lean_ctor_set_usize(ret, 1, 0);
+  lean_ctor_set_usize(ret, 2, size);
+  return lean_io_result_mk_ok(ret);
+}
+
+LEAN_EXPORT lean_obj_res lean_sodium_randombytes_buf_refresh(b_lean_obj_arg tau, lean_obj_arg buf, lean_obj_arg world) {
+  size_t size = lean_ctor_get_usize(buf, 2);
+  void* ptr = secure_obj_of_lean(lean_ctor_get(buf, 0));
+  sodium_mprotect_readwrite(ptr);
+  randombytes_buf(ptr, size);
+  sodium_mprotect_readonly(ptr);
+  lean_ctor_set_usize(buf, 1, 0);
+  return buf;
+}
+
+LEAN_EXPORT lean_obj_res lean_sodium_randombytes_buf_refresh_deterministic(b_lean_obj_arg tau, lean_obj_arg buf, b_lean_obj_arg seed, lean_obj_arg world) {
+  size_t size = lean_ctor_get_usize(buf, 2);
+  void* ptr = secure_obj_of_lean(lean_ctor_get(buf, 0));
+  sodium_mprotect_readwrite(ptr);
+  randombytes_buf_deterministic(ptr, size, lean_sarray_cptr(seed));
+  sodium_mprotect_readonly(ptr);
+  lean_ctor_set_usize(buf, 1, 0);
+  return buf;
+}
+
+LEAN_EXPORT lean_obj_res lean_sodium_randombytes_buf_extract_slice(b_lean_obj_arg tau, lean_obj_arg buf, size_t len, lean_obj_arg world) {
+  size_t off = lean_ctor_get_usize(buf, 1);
+  size_t size = lean_ctor_get_usize(buf, 2);
+  len = (off >= size) ? 0 : (off + len > size) ? (size - off) : len;
+
+  if (len == 0) {
+    lean_obj_res pair = lean_alloc_ctor(0, 2, 0);
+    lean_ctor_set(pair, 0, lean_alloc_sarray(sizeof(uint8_t), 0, 0));
+    lean_ctor_set(pair, 1, buf);
+    return pair;
+  }
+
+  lean_object* out = lean_alloc_sarray(sizeof(uint8_t), len, len);
+  uint8_t* ptr = secure_obj_of_lean(lean_ctor_get(buf, 0));
+  memcpy(lean_sarray_cptr(out), ptr + off, len);
+  sodium_mprotect_readwrite(ptr);
+  sodium_memzero(ptr + off, len);
+  sodium_mprotect_readonly(ptr);
+  lean_ctor_set_usize(buf, 1, off + len);
+  lean_object* pair = lean_alloc_ctor(0, 2, 0);
+  lean_ctor_set(pair, 0, out);
+  lean_ctor_set(pair, 1, buf);
+  return pair;
+}
+
+LEAN_EXPORT uint8_t lean_sodium_bytes_compare(size_t size, b_lean_obj_arg bytes1, b_lean_obj_arg bytes2) {
+  return sodium_compare(lean_sarray_cptr(bytes1), lean_sarray_cptr(bytes2), size) + 1;
+}
+
+LEAN_EXPORT uint8_t lean_sodium_bytes_dec_eq(size_t size, b_lean_obj_arg bytes1, b_lean_obj_arg bytes2) {
+  return sodium_compare(lean_sarray_cptr(bytes1), lean_sarray_cptr(bytes2), size) == 0;
+}
+
+LEAN_EXPORT uint8_t lean_sodium_bytes_dec_lt(size_t size, b_lean_obj_arg bytes1, b_lean_obj_arg bytes2) {
+  return sodium_compare(lean_sarray_cptr(bytes1), lean_sarray_cptr(bytes2), size) == -1;
+}
+
+LEAN_EXPORT lean_obj_res lean_sodium_bytes_to_base64(b_lean_obj_arg buf) {
+  size_t len = lean_sarray_size(buf);
+  size_t maxlen = sodium_base64_encoded_len(len, sodium_base64_VARIANT_URLSAFE);
+  lean_object* b64 = lean_alloc_string(1, maxlen, 0);
+  sodium_bin2base64(lean_to_string(b64)->m_data, maxlen, lean_sarray_cptr(buf), len, sodium_base64_VARIANT_URLSAFE);
+  len = strlen(lean_to_string(b64)->m_data);
+  lean_to_string(b64)->m_size = len + 1;
+  lean_to_string(b64)->m_length = len;
+  return b64;
+}
+
+LEAN_EXPORT lean_obj_res lean_sodium_bytes_of_base64(b_lean_obj_arg str) {
+  size_t size = lean_string_size(str);
+  size_t maxlen = size / 4 * 3 + 1;
+  size_t binlen;
+  lean_object* bin = lean_alloc_sarray(sizeof(uint8_t), maxlen, maxlen);
+
+  if (sodium_base642bin(lean_sarray_cptr(bin), maxlen, lean_string_cstr(str), size, " \r\n\t", &binlen, NULL, sodium_base64_VARIANT_URLSAFE) != 0) {
+    lean_dec(bin);
+    return lean_box(0);
+  }
+
+  lean_sarray_set_size(bin, binlen);
+  lean_object* some = lean_alloc_ctor(1, 1, 0);
+  lean_ctor_set(some, 0, bin);
+  return some;
+}
+
+LEAN_EXPORT lean_obj_res lean_sodium_bytes_increment(lean_obj_arg bytes, lean_obj_arg world) {
+  sodium_increment(lean_sarray_cptr(bytes), lean_sarray_size(bytes));
+  return bytes;
+}
+
+LEAN_EXPORT lean_obj_res lean_sodium_bytes_increment_vec(size_t n, lean_obj_arg bytes, lean_obj_arg world) {
+  sodium_increment(lean_sarray_cptr(bytes), lean_sarray_size(bytes));
+  return bytes;
+}
