ffi/generichash.c
@@ -1,0 +1,78 @@
+#include "ffi.h"
+
+LEAN_EXPORT lean_obj_res lean_sodium_generichash(b_lean_obj_arg input, b_lean_obj_arg key) {
+  lean_object* data;
+  uint8_t* ptr = NULL;
+  size_t len = 0;
+
+  if (!lean_is_scalar(key)) {
+    data = lean_ctor_get(key, 0);
+    ptr = lean_sarray_cptr(data);
+    len = lean_sarray_size(data);
+  }
+
+  lean_object* ret = lean_alloc_sarray(
+    sizeof(uint8_t),
+    crypto_generichash_BYTES_MAX,
+    crypto_generichash_BYTES_MAX);
+
+  crypto_generichash(
+    lean_sarray_cptr(ret),
+    lean_sarray_size(ret),
+    lean_sarray_cptr(input),
+    lean_sarray_size(input),
+    ptr,
+    len);
+
+  return ret;
+}
+
+LEAN_EXPORT lean_obj_res lean_sodium_generichash_init(b_lean_obj_arg key) {
+  lean_object* data;
+  uint8_t* ptr = NULL;
+  size_t len = 0;
+
+  if (!lean_is_scalar(key)) {
+    data = lean_ctor_get(key, 0);
+    ptr = lean_sarray_cptr(data);
+    len = lean_sarray_size(data);
+  }
+
+  lean_object* state = lean_alloc_sarray(
+    sizeof(uint8_t),
+    sizeof(crypto_generichash_state),
+    sizeof(crypto_generichash_state));
+
+  crypto_generichash_init(
+    (crypto_generichash_state*) lean_sarray_cptr(state),
+    ptr,
+    len,
+    crypto_generichash_BYTES_MAX);
+
+  lean_object* stream = lean_alloc_ctor(0, 1, 0);
+  lean_ctor_set(stream, 0, state);
+  return stream;
+}
+
+LEAN_EXPORT lean_obj_res lean_sodium_generichash_update(lean_obj_arg stream, b_lean_obj_arg input) {
+  crypto_generichash_update(
+    (crypto_generichash_state*) lean_sarray_cptr(lean_ctor_get(stream, 0)),
+    lean_sarray_cptr(input),
+    lean_sarray_size(input));
+
+  return stream;
+}
+
+LEAN_EXPORT lean_obj_res lean_sodium_generichash_final(b_lean_obj_arg stream) {
+  lean_object* ret = lean_alloc_sarray(
+    sizeof(uint8_t),
+    crypto_generichash_BYTES_MAX,
+    crypto_generichash_BYTES_MAX);
+
+  crypto_generichash_final(
+    (crypto_generichash_state*) lean_sarray_cptr(lean_ctor_get(stream, 0)),
+    lean_sarray_cptr(ret),
+    crypto_generichash_BYTES_MAX);
+
+  return ret;
+}
