ffi/kdf.c
@@ -1,0 +1,20 @@
+#include "ffi.h"
+
+LEAN_EXPORT lean_obj_res lean_sodium_kdf_derive_from_key(b_lean_obj_arg tau, uint64_t idx, b_lean_obj_arg ctx, b_lean_obj_arg key, lean_obj_arg world) {
+  void* ptr = sodium_malloc(32);
+  void* mptr = secure_obj_of_lean(lean_ctor_get(key, 0));
+  sodium_mprotect_readonly(mptr);
+  int err = crypto_kdf_blake2b_derive_from_key(ptr, 32, idx, (const char*) lean_sarray_cptr(ctx), mptr);
+  sodium_mprotect_noaccess(ptr);
+  sodium_mprotect_noaccess(mptr);
+
+  if (err != 0) {
+    sodium_free(ptr);
+    return lean_io_result_mk_error(lean_mk_io_user_error(lean_mk_string("crypto_kdf_blake2b_derive_from_key failed")));
+  }
+
+  lean_object* ret = lean_alloc_ctor(0, 1, sizeof(size_t));
+  lean_ctor_set(ret, 0, secure_obj_to_lean(ptr));
+  lean_ctor_set_usize(ret, 1, 32);
+  return lean_io_result_mk_ok(ret);
+}
