Sodium/Data/ByteVector.lean
@@ -1,15 +1,9 @@
-import Sodium.Data.ByteArray
-import Sodium.Data.Encodable.Basic
-
-open Lean Alloy.C
-
-alloy c include <lean/lean.h> <sodium.h> <string.h>
-
 structure ByteVector (n : Nat) where
-  toArray : ByteArray
-  size_toArray : toArray.size = n
+  toByteArray : ByteArray
+  size_toByteArray : toByteArray.size = n
+  deriving DecidableEq
 
-attribute [simp, grind] ByteVector.size_toArray
+attribute [simp, grind =] ByteVector.size_toByteArray
 
 variable {n m : Nat}
 
@@ -28,152 +22,71 @@ def empty : ByteVector 0 := ⟨ByteArray.empty, rfl⟩
 instance : EmptyCollection (ByteVector 0) where
   emptyCollection := ⟨ByteArray.empty, rfl⟩
 
-def push : ByteVector n → UInt8 → ByteVector (n + 1)
-  | ⟨bs, h⟩, b => ⟨bs.push b, by simpa [ByteArray.size_push]⟩
-
-def usize (_ : ByteVector n) : USize := n
-
-alloy c extern "lean_sodium_increment_vec"
-def succ (buf : @& ByteVector n) : ByteVector n :=
-  size_t len = lean_sarray_size(buf);
-  uint8_t* buf_ptr = lean_sarray_cptr(buf);
-  lean_object* out = lean_alloc_sarray(sizeof(uint8_t), len, len);
-  uint8_t* out_ptr = lean_sarray_cptr(out);
-  memcpy(out_ptr, buf_ptr, len);
-  sodium_increment(out_ptr, len);
-  return out;
-
-def isZero (x : ByteVector n) : Bool := x.toArray.isZero
-
--- def uget : (a : ByteVector n) → (i : USize) → (h : i < n := by get_elem_tactic) → UInt8
---   | ⟨bs, hb⟩, i, h => bs[i]'(by
---     rw [USize.toFin_val]
---     refine (USize.lt_ofNat_iff ?_).mp ?_
---     · exact ByteArray.size_lt_USize_size bs
---     · rw [← Nat.toUSize_eq, ← ByteArray.usize, hb]
---       exact h)
-
-def get! : (ByteVector n) → Nat → UInt8
-  | ⟨bs, _⟩, i => bs[i]!
-
-def get : (a : ByteVector n) → (i : Nat) → (h : i < n := by get_elem_tactic) → UInt8
-  | ⟨bs, hb⟩, i, h => bs[i]'(by
-    refine Nat.lt_of_le_of_ne ?_ ?_
-    . subst hb
-      simp_all only [gt_iff_lt]
-      exact Nat.le_of_succ_le h
-    . subst hb
-      simp_all only [gt_iff_lt]
-      intro a
-      subst a
-      simp_all only [Nat.lt_irrefl]
-  )
-
-instance : GetElem (ByteVector n) Nat UInt8 fun _ i => i < n where
-  getElem xs i _ := xs.get i
-
--- instance : GetElem (ByteVector n) USize UInt8 fun _ i => i.toFin < n where
---   getElem xs i h := xs.uget i (by sorry)
-
-def set! : (ByteVector n) → Nat → UInt8 → ByteVector n
-  | ⟨bs, hb⟩, i, b => ⟨bs.set! i b, by simp [ByteArray.set!, ByteArray.size]; rw [← hb]; rfl⟩
-
-def set : (a : ByteVector n) → (i : Nat) → UInt8 → (h : i < n := by get_elem_tactic) → ByteVector n
-  | ⟨bs, hb⟩, i, b, h => ⟨bs.set i b (by subst hb; simp_all only [gt_iff_lt]), by simp [ByteArray.set, ByteArray.size]; rw [← hb]; rfl⟩
-
--- def uset : (a : ByteVector n) → (i : USize) → UInt8 → (h : i < n := by get_elem_tactic) → ByteVector n
---   | ⟨bs, hb⟩, i, v, h => ⟨bs.uset i v (by sorry), by simp [ByteArray.uset, ByteArray.size]; rw [← hb]; rfl⟩
-
-protected abbrev hash (a : ByteVector n) : UInt64 := a.toArray.hash
+protected abbrev hash (a : ByteVector n) : UInt64 := a.toByteArray.hash
 
 instance : Hashable (ByteVector n) where
   hash := ByteVector.hash
 
--- def extract (a : ByteVector n) (b e : Nat) : ByteVector (min n e - b) where
---   toArray := a.toArray.copySlice b .empty 0 (e - b)
---   usize_toArray := by
---     simp [ByteArray.copySlice, ByteArray.usize, ByteArray.size]
---     sorry
+@[extern "lean_sodium_bytes_compare"]
+opaque compare (x y : @& ByteVector n) : Ordering
 
-protected def append {n m : Nat} (a : ByteVector n) (b : ByteVector m) : ByteVector (n + m) where
-  toArray := b.toArray.copySlice 0 a.toArray n m false
-  size_toArray := by
-    simp [ByteArray.copySlice, ByteArray.size]
-    rw [← ByteArray.size, ← ByteArray.size]
-    rw [a.size_toArray, b.size_toArray]
-    simp only [Nat.min_self]
-    omega
+instance : Ord (ByteVector n) := ⟨compare⟩
+instance : BEq (ByteVector n) := ⟨(compare · · == .eq)⟩
+instance : LT (ByteVector n) := ⟨(compare · · == .lt)⟩
 
-instance {n m : Nat} : HAppend (ByteVector n) (ByteVector m) (ByteVector (n + m)) :=
-  ⟨ByteVector.append⟩
+@[extern "lean_sodium_bytes_dec_eq"]
+def decEq (x y : @& ByteVector n) : Decidable (Eq x y) :=
+  match x, y with
+  | ⟨⟨⟨x⟩⟩, _⟩, ⟨⟨⟨y⟩⟩, _⟩ =>
+    dite (x = y)
+      (fun h => match x, y, h with | _, _, Eq.refl _ => isTrue rfl)
+      (fun h => isFalse (fun h' => h (congrArg (fun z => Array.toList z.toByteArray.data) h')))
 
+@[extern "lean_sodium_bytes_dec_lt"]
+def decLt (x y : @& ByteVector n) : Decidable (LT.lt x y) :=
+  dite (compare x y == .lt) isTrue isFalse
+
+instance : DecidableEq (ByteVector n) := decEq
+instance : DecidableLT (ByteVector n) := decLt
 instance {n m : Nat} {h : n = m} : HEq (ByteVector n) (ByteVector m) := by subst h; rfl
 
-def toList (bs : ByteVector n) : List UInt8 := bs.toArray.toList
+def toArray (bs : ByteVector n) : Array UInt8 := bs.toByteArray.data
+def toList (bs : ByteVector n) : List UInt8 := bs.toByteArray.toList
 
 @[inline] def findIdx? (x : ByteVector n) (p : UInt8 → Bool) (start := 0) : Option Nat :=
-  x.toArray.findIdx? p start
+  x.toByteArray.findIdx? p start
 
 @[inline] protected def cast (h : n = m := by native_decide) (x : ByteVector n) : ByteVector m :=
-  ⟨x.toArray, by rw [← h]; exact x.size_toArray⟩
+  ⟨x.toByteArray, by rw [← h]; exact x.size_toByteArray⟩
 
 @[inline] def cast? (x : ByteVector n) : Option (ByteVector m) :=
-  if h : n = m then
-    some ⟨x.toArray, by rw [← h]; exact x.size_toArray⟩
-  else
-    none
+  if h : n = m then some ⟨x.toByteArray, by rw [← h]; exact x.size_toByteArray⟩
+  else none
 
 instance {n m : Nat} {h : n = m} : ∀ x : ByteVector n, HEq (x.cast h) x := fun _ => by subst h; rfl
 
 @[inline] def findFinIdx? (a : ByteVector n) (p : UInt8 → Bool) (start := 0) : Option (Fin n) :=
-  let b := a.toArray.findFinIdx? p start
-  a.size_toArray ▸ b
+  let b := a.toByteArray.findFinIdx? p start
+  a.size_toByteArray ▸ b
 
-abbrev toBase64 (bs : ByteVector n) : String := bs.toArray.toBase64
-
-def ofBase64? (s : String) : Option (ByteVector n) := do
-  let data ← ByteArray.ofBase64? s
-  if h : data.size = n then some ⟨data, h⟩
-  else none
-
-abbrev toUInt64LE (bs : ByteVector 8) : UInt64 := bs.toArray.toUInt64LE!
-abbrev toUInt64BE (bs : ByteVector 8) : UInt64 := bs.toArray.toUInt64BE!
-
-instance : ToJson (ByteVector n) := ⟨toJson ∘ ByteVector.toArray⟩
-
-instance : FromJson (ByteVector n) where
-  fromJson? json := do
-    let bs ← fromJson? (α := ByteArray) json
-    if h : bs.size = n then return ⟨bs, h⟩
-    else throw s!"expected exactly {n} bytes"
-
-instance : BEq (ByteVector n) where
-  beq x y := compare x.toArray y.toArray == .eq
-
-instance : Ord (ByteVector n) := ⟨fun x y => compare x.toArray y.toArray⟩
-instance : LT (ByteVector n) := ⟨fun x y => x.toArray < y.toArray⟩
-
-instance : DecidableLT (ByteVector n) := by
-  intro x y
-  by_cases h : x.toArray < y.toArray
-  . exact isTrue h
-  . exact isFalse h
+abbrev toUInt64LE (bs : ByteVector 8) : UInt64 := bs.toByteArray.toUInt64LE!
+abbrev toUInt64BE (bs : ByteVector 8) : UInt64 := bs.toByteArray.toUInt64BE!
 
 end ByteVector
 
 namespace ByteArray
 
-abbrev toVector (bs : ByteArray) : ByteVector bs.size := .mk bs rfl
+abbrev toByteVector (bs : ByteArray) : ByteVector bs.size := .mk bs rfl
 
-abbrev toVector? (bs : ByteArray) : Option (ByteVector n) :=
+abbrev toByteVector? (bs : ByteArray) : Option (ByteVector n) :=
   if h : bs.size = n then some ⟨bs, h⟩
   else none
 
 abbrev toVector! (bs : ByteArray) : ByteVector n :=
-  bs.toVector?.get!
+  bs.toByteVector?.get!
 
-@[simp] theorem toVector_size : ∀ bs : ByteArray, bs.toVector.size = bs.size := by intro; rfl
-@[simp] theorem toVector_inj : ∀ bs : ByteArray, bs.toVector.toArray = bs := by intro; rfl
+@[simp, grind =] theorem toByteVector_size : ∀ bs : ByteArray, bs.toByteVector.size = bs.size := by intro; rfl
+@[simp] theorem toByteVector_inj : ∀ bs : ByteArray, bs.toByteVector.toByteArray = bs := by intro; rfl
 
 end ByteArray
 
@@ -181,18 +94,7 @@ namespace ByteVector
 
 variable {n : Nat}
 
-@[simp] theorem toArray_inj : ∀ bs : ByteVector n, bs.toArray.toVector = bs.cast (by exact Eq.symm bs.size_toArray) := by intro; rfl
-
-instance : DecidableEq (ByteVector n) := fun a b =>
-  match decEq a.toArray b.toArray with
-  | isTrue h => isTrue (by cases a; cases b; simp_all only)
-  | isFalse h => isFalse fun eq => by cases eq; exact h rfl
-
-instance : Encodable (ByteVector n) :=
-  Encodable.ofLeftInj (·.toArray) (·.toVector.cast?) fun x => by
-    simp only [toArray_inj]
-    unfold cast?
-    simp only [size_toArray, ↓reduceDIte, Option.some.injEq]
-    rfl
+@[simp] theorem toByteArray_inj : ∀ bs : ByteVector n, bs.toByteArray.toByteVector = bs.cast (by exact Eq.symm bs.size_toByteArray) :=
+  by intro; rfl
 
 end ByteVector
