Sodium/Data/Decrypt.lean
@@ -1,0 +1,84 @@
+import Sodium.Data.Encodable
+
+namespace Sodium
+
+inductive Decrypt (α)
+  | refused
+  | mangled (data : ByteArray)
+  | unknown (string : String)
+  | almost (json : Lean.Json)
+  | accepted (a : α)
+
+namespace Decrypt
+
+inductive Error
+  | refused
+  | invalidEncoding (data : ByteArray)
+  | invalidString (string : String)
+  | invalidJson (json : Lean.Json)
+  deriving TypeName, Hashable, Inhabited
+
+variable {α}
+
+@[coe]
+def toExcept : Decrypt α → Except Error α
+| .refused => .error .refused
+| .mangled data => .error (.invalidEncoding data)
+| .unknown string => .error (.invalidString string)
+| .almost json => .error (.invalidJson json)
+| .accepted a => .ok a
+
+@[coe]
+def ofExcept : Except Error α → Decrypt α
+| .error .refused => .refused
+| .ok a => .accepted a
+| .error (.invalidEncoding data) => .mangled data
+| .error (.invalidString string) => .unknown string
+| .error (.invalidJson json) => .almost json
+
+instance : Coe (Decrypt α) (Except Error α) := ⟨toExcept⟩
+instance : Coe (Except Error α) (Decrypt α) := ⟨ofExcept⟩
+
+@[simp]
+theorem toExcept_inj : ∀ r : Except Error α, toExcept (ofExcept r) = r := by
+  intro
+  unfold toExcept ofExcept
+  split <;> next _ _ h => split at h <;> simp_all
+
+@[simp]
+theorem ofExcept_inj : ∀ r : Decrypt α, ofExcept (toExcept r) = r := by
+  intro
+  unfold ofExcept toExcept
+  split <;> next _ _ h => split at h <;> simp_all
+
+@[simp]
+theorem toExcept_ok_iff {a : α} : ∀ r : Decrypt α, toExcept r = .ok a ↔ r = .accepted a := by
+  intro
+  unfold toExcept
+  constructor
+  · intro a
+    split at a <;> next _ _ => simp_all
+  · intro a
+    subst a
+    simp_all only
+
+variable (α) [Encodable α]
+
+def ofJson (json : Lean.Json) : Decrypt α :=
+  match decode? (α := α) json with
+  | .some a => .accepted a
+  | _ => .almost json
+
+def ofString (string : String) : Decrypt α :=
+  match Lean.Json.parse string with
+  | .ok json => ofJson _ json
+  | _ => .unknown string
+
+def ofByteArray (data : ByteArray) : Decrypt α :=
+  match String.fromUTF8? data with
+  | .some string => ofString _ string
+  | _ => .mangled data
+
+end Decrypt
+
+end Sodium
