Sodium/Data/SecretVector.lean
@@ -1,0 +1,71 @@
+import Sodium.Init
+import Sodium.Data.ByteVector
+
+universe u
+
+opaque SecurePointed : NonemptyType
+
+namespace Sodium
+
+structure SecretVector {σ} (_ : Sodium σ) (n : USize) where
+  private mk ::
+  private ref : SecurePointed.type
+  usize : USize
+  usize_rfl : usize = n
+
+namespace SecretVector
+
+variable {σ} {τ : @& Sodium σ}
+
+noncomputable instance {n} : Nonempty (τ.SecretVector n) :=
+  ⟨{ ref := Classical.choice SecurePointed.property, usize := n, usize_rfl := rfl }⟩
+
+@[extern "lean_sodium_malloc"]
+opaque randomBytes (n : USize) : IO (τ.SecretVector n)
+
+@[extern "lean_sodium_malloc_deterministic"]
+opaque seededBytes (n : USize) (seed : @& ByteVector 32) : IO (τ.SecretVector n)
+
+@[extern "lean_sodium_secure_obj_is_zero"]
+opaque isZero {n} (obj : @& τ.SecretVector n) : Bool
+
+@[extern "lean_sodium_secure_obj_compare"]
+opaque compare {n} (obj1 obj2 : @& τ.SecretVector n) : Ordering
+
+instance {n} : Ord (τ.SecretVector n) := ⟨compare⟩
+instance {n} : BEq (τ.SecretVector n) := ⟨(compare · · == .eq)⟩
+instance {n} : LT (τ.SecretVector n) := ⟨(compare · · == .lt)⟩
+
+end SecretVector
+
+structure Entropy {σ} (_ : Sodium σ) where
+  private mk ::
+  private ref : SecurePointed.type
+  uoff : USize
+  usize : USize
+
+namespace Entropy
+
+variable {σ} {τ : @& Sodium σ}
+
+noncomputable instance : Nonempty τ.Entropy :=
+  ⟨{ ref := Classical.choice SecurePointed.property, uoff := 0, usize := 0 }⟩
+
+@[extern "lean_sodium_randombytes_buf"]
+opaque randomBytes (n : USize) : IO τ.Entropy
+
+@[extern "lean_sodium_randombytes_buf_deterministic"]
+opaque seededBytes (n : USize) (seed : @& ByteVector 32) : IO τ.Entropy
+
+@[extern "lean_sodium_randombytes_buf_refresh"]
+opaque refresh (bytes : τ.Entropy) : BaseIO τ.Entropy
+
+@[extern "lean_sodium_randombytes_buf_refresh_deterministic"]
+opaque seededRefresh (bytes : τ.Entropy) (seed : @& ByteVector 32) : BaseIO τ.Entropy
+
+@[extern "lean_sodium_randombytes_buf_extract_slice"]
+opaque extractSlice (bytes : τ.Entropy) (n : USize) : BaseIO (ByteArray × τ.Entropy)
+
+end Entropy
+
+end Sodium
